#+TITLE: knowledge repo
#+SUBTITLE: Mathematics Topics
#+INCLUDE: "../navbar.html" export html
#+OPTIONS: toc:nil
#+OPTIONS: num:nil
#+HEADER: :results output silent :headers '("\\usepackage{tikz}")

* Arithmetic Progression
  The mathematician Johann Faulhaber was able to elegantly express in the
  17th-century the result of the following sum:
  \[\sum_{k=1}^n k^p = 1^p+ 2^p+3^p+...+n^p\]
  for $n>0$ and $p>0$
  
  The very result is not the point but rather what insights we can draw from it.
  Let's start from unpretentiously, and assuming $p=1$:
  \[\sum_{k=1}^n k^1 = 1+ 2+3+...+n\]

  The solution to this one is well-known to be $(n+1)n/2$ by doing the trick of
  adding $1$ to $n$, 2 to $n-1$, and then counting the amount of $n+1$ terms there is.
  But what if $p=2$?
  \[\sum_{k=1}^n k^2 = 1^2+ 2^2+3^2+...+n^2\]

  In this case this old trick won't work, as $n^2+1 \ne (n-1)^2+2 = n^2-2n+3$ in
  this case and in the case for bigger values of $p$ we can get the sum by the
  binomial formula then summing each side of the equation.
  \[(n-1)^3 = n^3 - 3n^2 + 3n - 1 \\
    (n-1)^3 - n^3 = 3n^2 + 3n - 1 \\
    \sum_{k=1}^n (k-1)^3 - k^3 = -\sum_{k=1}^n 3k^2 + 3k - 1\]

  The advantage of using this method, is the convenient shape of the terms in the
  left-hand side $\sum (u-1)^p - u^p$ which will cancel neighboring terms leaving only those
  in the extremes:
  \[\sum_{k=1}^n (k-1)^3 - k^3 = (0 - 1) + (1 - 2^3) + (2^3 - 3^3) + ... + ((n-2)^3 - (n-1)^3) + ((n-1)^3 - n^3) \\
    \sum_{k=1}^n (k-1)^3 - k^3 = - n^3\]

  Distributing the sum operator to each term in the right-hand side:  $-3\sum_{k=1}^n k^2 + \sum_{k=1}^n k - n$

  As one can use the old trick to get the value of $\sum_{k=1}^n k$ we can write
  the whole equation in the following form:
  \[\sum_{k=1}^n k^2 = \frac{2n^3 + 3n(n+1) - 2n}{6} = \frac{n(2n^2 + 3n + 1)}{6}\]
  
    
